Weidenbach_Book/IsaSAT/IsaSAT_Simplify_Pure_Literals_LLVM.thy
@@ -87,9 +87,9 @@ sepref_def isa_pure_literal_deletion_wl_code
   :: \<open>[\<lambda>(_, S). length (get_clauses_wl_heur S) \<le> sint64_max \<and> learned_clss_count S \<le> uint64_max]\<^sub>a
      (larray_assn' TYPE(64) bool1_assn)\<^sup>d *\<^sub>a isasat_bounded_assn\<^sup>d \<rightarrow> word64_assn \<times>\<^sub>a isasat_bounded_assn\<close>
   unfolding isa_pure_literal_deletion_wl_alt_def nres_monad3 nres_monad2
-    get_vmtf_heur_array_nth_def[symmetric] UNSET_def[symmetric] atom.fold_option
+    get_bump_heur_array_nth_def[symmetric] UNSET_def[symmetric] atom.fold_option
     mop_polarity_st_heur_def[symmetric] tri_bool_eq_def[symmetric]
-    get_vmtf_heur_array_nth_def[symmetric] prod.simps
+    get_bump_heur_array_nth_def[symmetric] prod.simps
   by sepref
 
 end
